python/Demo2-py/module_.py
@@ -1,0 +1,12 @@
+import sys
+from typing import Callable, Any, TypeVar, NamedTuple
+from math import floor
+from itertools import count
+
+import module_ as module_
+import _dafny as _dafny
+import System_ as System_
+import M as M
+
+# Module: module_
+
