python/Demo2x.py
@@ -1,0 +1,7 @@
+import M
+
+def main():
+    print("Hi");
+    M.C.p();
+
+main()
