python/yaml_to_obj-py/YamlToDafnyTranslator.py
@@ -1,0 +1,27 @@
+import sys
+from typing import Callable, Any, TypeVar, NamedTuple
+from math import floor
+from itertools import count
+
+import module_ as module_
+import _dafny as _dafny
+import System_ as System_
+
+# Module: YamlToDafnyTranslator
+
+class default__:
+    def  __init__(self):
+        pass
+
+    @staticmethod
+    def Main(args):
+        if (len(args)) < (2):
+            return
+        d_0_path_: _dafny.Seq
+        d_0_path_ = (args)[1]
+        d_1_content_: _dafny.Seq
+        out0_: _dafny.Seq
+        out0_ = FileUtils.ReadAllLines(d_0_path_)
+        d_1_content_ = out0_
+        FileUtils.WriteLine(_dafny.SeqWithoutIsStrInference(map(_dafny.CodePoint, "Read lines from file")))
+
