python/yaml_to_obj-py/__main__.py
@@ -1,0 +1,16 @@
+# Dafny program yaml_to_obj.dfy compiled into Python
+import sys
+from typing import Callable, Any, TypeVar, NamedTuple
+from math import floor
+from itertools import count
+
+import module_ as module_
+import _dafny as _dafny
+
+import YamlToDafnyTranslator
+try:
+    dafnyArgs = [_dafny.SeqWithoutIsStrInference(map(_dafny.CodePoint, a)) for a in sys.argv]
+    YamlToDafnyTranslator.default__.Main(dafnyArgs)
+except _dafny.HaltException as e:
+    _dafny.print("[Program halted] " + e.message + "\n")
+    sys.exit(1)
